% !TEX program = pdflatex
\documentclass[10pt]{article}
\usepackage[margin=0.75in]{geometry}
\usepackage{amsmath,amssymb}
\usepackage[T1]{fontenc}
\usepackage{mathptmx}
\setlength{\parindent}{0pt}
\setlength{\parskip}{4pt}

\begin{document}
{\bf MATH 266 -- HW 10 Solutions (Problems 1, 3, 5)}

\small

\textbf{Problem 1.} Solve $\vec x' = A\vec x$, $\vec x(0)=\binom{1}{1}$, where
\[
A=\begin{pmatrix}1&5\\[2pt]1&-3\end{pmatrix}.
\]

The characteristic polynomial is
\[
\det(A-\lambda I)=\lambda^2+2\lambda-8=(\lambda+4)(\lambda-2),
\]
so $\lambda_1=-4$, $\lambda_2=2$.

For $\lambda_1=-4$, $(A+4I)\vec v_1=0$ gives $x_1+x_2=0$, so take
\[
\vec v_1=\binom{1}{-1}.
\]
For $\lambda_2=2$, $(A-2I)\vec v_2=0$ gives $-x_1+5x_2=0$, so take
\[
\vec v_2=\binom{5}{1}.
\]

Thus the general solution is
\[
\vec x(t)=C_1e^{-4t}\binom{1}{-1}+C_2e^{2t}\binom{5}{1}.
\]
Using $\vec x(0)=\binom{1}{1}$,
\[
C_1\binom{1}{-1}+C_2\binom{5}{1}=\binom{1}{1}
\quad\Rightarrow\quad
C_1=-\tfrac23,\; C_2=\tfrac13.
\]
Hence
\[
\boxed{\;\vec x(t)=-\frac23 e^{-4t}\binom{1}{-1}+\frac13 e^{2t}\binom{5}{1}\;}
\]

\textbf{Problem 3.} Solve $\vec x' = A\vec x$, where
\[
A=\begin{pmatrix}1&1&2\\[2pt]1&2&1\\[2pt]2&1&1\end{pmatrix}.
\]

The eigenvalues are $\lambda=1,4,-1$ with eigenvectors
\[
\vec v_1=\begin{pmatrix}1\\-2\\1\end{pmatrix},\quad
\vec v_2=\begin{pmatrix}1\\1\\1\end{pmatrix},\quad
\vec v_3=\begin{pmatrix}-1\\0\\1\end{pmatrix}.
\]
Thus
\[
\boxed{\;\vec x(t)=C_1 e^{t}\!\begin{pmatrix}1\\-2\\1\end{pmatrix}
+ C_2 e^{4t}\!\begin{pmatrix}1\\1\\1\end{pmatrix}
+ C_3 e^{-t}\!\begin{pmatrix}-1\\0\\1\end{pmatrix}\;}
\]

\textbf{Problem 5.} Solve $\vec x' = A\vec x$, where
\[
A=\begin{pmatrix}1&2&-1\\[2pt]0&1&1\\[2pt]0&-1&1\end{pmatrix}.
\]

The eigenvalues are $\lambda=1$, $1\pm i$.
An eigenvector for $\lambda=1$ is $\binom{1}{0}{0}$.
For $\lambda=1+i$, take
\[
\vec v=\begin{pmatrix}-1-2i\\[2pt]1\\[2pt]i\end{pmatrix}
=\vec a+i\vec b,
\quad
\vec a=\begin{pmatrix}-1\\1\\0\end{pmatrix},
\;
\vec b=\begin{pmatrix}-2\\0\\1\end{pmatrix}.
\]
Real solutions are
\[
\vec x_2(t)=e^{t}\!\begin{pmatrix}-\cos t+2\sin t\\ \cos t\\ -\sin t\end{pmatrix},
\quad
\vec x_3(t)=e^{t}\!\begin{pmatrix}-2\cos t-\sin t\\ \sin t\\ \cos t\end{pmatrix}.
\]
Hence
\[
\boxed{\;\vec x(t)=C_1 e^{t}\!\begin{pmatrix}1\\0\\0\end{pmatrix}
+ C_2 e^{t}\!\begin{pmatrix}-\cos t+2\sin t\\ \cos t\\ -\sin t\end{pmatrix}
+ C_3 e^{t}\!\begin{pmatrix}-2\cos t-\sin t\\ \sin t\\ \cos t\end{pmatrix}\;}
\]

\end{document}